arrays/spec/contains.v
@@ -1,0 +1,139 @@
+From Coq Require Import Sorting.Sorted.
+
+From iris.algebra Require Import auth frac_auth gset.
+From iris.heap_lang Require Import proofmode.
+
+From SkipList.lib Require Import lock misc node_rep node_lt key_equiv.
+From SkipList.arrays Require Import code.
+From SkipList.arrays.inv Require Import list_equiv lazy_inv skip_inv.
+From SkipList.arrays.spec Require Import find.
+
+
+Local Open Scope Z.
+
+Module ContainsSpec (Params: SKIP_LIST_PARAMS).
+  Import Params.
+  Module Find := FindSpec Params.
+  Export Find.
+
+  Section Proofs.
+    Context `{!heapGS Σ, !gset_list_unionGS Σ, !lockG Σ}.
+    
+    Theorem findPred_spec (key lvl: Z) (top_head curr: node_rep) (Skeys: gset Z) 
+      (bot: bot_gname) (top_sub: sub_gname) (bot_subs: list sub_gname) :
+      {{{ 
+        skip_list_equiv lvl top_head Skeys 1 bot (top_sub :: bot_subs)
+        ∗
+        (⌜ curr = top_head ⌝ ∨ own (s_auth top_sub) (◯ {[ curr ]}))
+        ∗
+        ⌜ node_key curr < key < INT_MAX ⌝
+      }}}
+        findPred (rep_to_node curr) #key #lvl
+      {{{ pred succ, RET ((rep_to_node pred), (rep_to_node succ));
+        skip_list_equiv lvl top_head Skeys 1 bot (top_sub :: bot_subs)
+        ∗
+        ⌜ key ∈ Skeys ↔ node_key succ = key ⌝
+      }}}.
+    Proof.
+      iIntros (Φ) "(Hlist & Hown_curr & Hrange) HΦ".
+      iRevert (curr top_head lvl top_sub bot_subs) "Hlist Hown_curr Hrange HΦ".
+      iLöb as "IH".
+      iIntros (curr top_head lvl top_sub bot_subs) "Hlist #Hown_curr %Hrange HΦ".
+
+      wp_lam. wp_let. wp_let.
+      destruct bot_subs as [|bot_sub].
+      + iDestruct "Hlist" as "(%Hlvl & (Hown_frag & #Hinv))".
+        wp_apply (find_bot_spec with "[Hown_frag]").
+        { by iFrame "# ∗". }
+        iIntros (pred succ) "(Hown_frag & %Hpred_key & #Hown_pred & %Hkey_in_S)".
+
+        wp_pures. case_bool_decide; wp_if.
+        - iModIntro. iApply "HΦ". 
+          by iFrame "# ∗".
+        - exfalso; congruence.
+      + iDestruct "Hlist" as "(%Hlvl & #Hinv & Hmatch)".
+        unfold is_top_list.
+        wp_apply find_sub_spec.
+        { by iFrame "# ∗". }
+        iIntros (pred succ) "(%Hrange' & #Hown_pred & #Hown_succ & _)".
+
+        wp_pures. case_bool_decide; wp_if.
+        - exfalso; assert (lvl = 0) by congruence; lia.
+        - wp_bind (Fst _).
+          iInv (levelN lvl) as (S Skeys' L) "(Hinv_sub & _)" "Hclose".
+          iDestruct "Hinv_sub" as "(>%Hperm & >%Hsort & >%Hequiv & >Hown_auth & >Hown_toks & Hlist)".
+
+          iDestruct "Hown_pred" as "[%Heq | #Hown_pred]".
+          * wp_proj.
+            iMod ("Hclose" with "[Hlist Hown_auth Hown_toks]") as "_".
+            { iNext; iExists S, Skeys', L; by iFrame. }
+
+            iModIntro; wp_pures.
+            iApply ("IH" with "[$] [] [%]").
+            { by iLeft. }
+            { lia. }
+            iNext; iIntros (? ?) "(? & ?)".
+            iApply "HΦ". by iFrame "# ∗".
+          * iAssert ⌜ In pred L ⌝%I with "[Hown_auth]" as %Hin.
+            {
+              iDestruct (own_valid_2 with "Hown_auth Hown_pred") 
+                as %[Hvalid%gset_included]%auth_both_valid_discrete.
+              rewrite -elem_of_list_In Hperm elem_of_elements.
+              iPureIntro; set_solver.
+            }
+
+            rewrite list_equiv_invert_L; last done.
+            iDestruct "Hlist" as (s' succ' ? ? γ) "(>%Hsucc'_range & _ & Hpt' & #Hs' & Hlock & HP & Himp)".
+            iDestruct "HP" as"(>Hauth_pred & >Htoks_pred)".
+
+            assert ({[ pred ]} = {[ pred ]} ⋅ {[ pred ]}) as -> by set_solver.
+            iDestruct "Hauth_pred" as "(Hauth_pred & ?)".
+
+            wp_proj.
+            iPoseProof ("Himp" with "[$]") as "Hlist".
+            iMod ("Hclose" with "[Hlist Hown_auth Hown_toks]") as "_".
+            { iNext; iExists S, Skeys', L; by iFrame. }
+
+            iModIntro; wp_pures.
+            iApply ("IH" with "[$] [Hauth_pred] [%]").
+            { by iRight. }
+            { lia. }
+            iNext; iIntros (? ?) "(? & ?)".
+            iApply "HΦ". by iFrame "# ∗".
+    Qed.
+    
+    Theorem contains_spec (key: Z) (v: val) (S: gset Z) 
+      (bot: bot_gname) (subs: list sub_gname)
+      (Hrange: INT_MIN < key < INT_MAX) :
+      {{{ is_skip_list v S 1 bot subs }}}
+        contains v #key
+      {{{ (b: bool), RET #b; 
+        is_skip_list v S 1 bot subs
+        ∗
+        ⌜ if b then key ∈ S else key ∉ S ⌝
+      }}}.
+    Proof.
+      iIntros (Φ) "H HΦ".
+      iDestruct "H" as (h head) "(%Hv & Hpt & %Hmin & Hlist)".
+      wp_lam. wp_let. rewrite -Hv. wp_load. wp_let.
+      destruct subs as [|sub subs]; first by iExFalso.
+
+      wp_apply (findPred_spec with "[Hlist]").
+      { iFrame. iSplit. by iLeft. iPureIntro; lia. }
+
+      iIntros (pred succ) "(Hlist & %Hkey_in_S)".
+      wp_pures. wp_lam. wp_pures.
+      
+      iModIntro; case_bool_decide.
+      + iApply "HΦ". iSplit.
+        { iExists h, head; by iFrame. }
+        iPureIntro. 
+        rewrite Hkey_in_S; congruence.
+      + iApply "HΦ". iSplit. 
+        { iExists h, head; by iFrame. }
+        iPureIntro; intros Hin. 
+        rewrite Hkey_in_S in Hin; congruence.
+    Qed.
+
+  End Proofs.
+End ContainsSpec.
