arrays/spec/new.v
@@ -6,6 +6,8 @@ From SkipList.arrays Require Import code.
 From SkipList.arrays.inv Require Import list_equiv lazy_inv skip_inv.
 
 
+Local Open Scope Z.
+
 Module NewSpec (Params: SKIP_LIST_PARAMS).
   Import Params.
   Module Invariant := SkipListInv Params.
@@ -14,15 +16,15 @@ Module NewSpec (Params: SKIP_LIST_PARAMS).
   Section Proofs.
     Context `{!heapGS Σ, !gset_list_unionGS Σ, !lockG Σ}.
 
-    Theorem array_inv (lvl: nat) (head: node_rep) (t: loc)
+    Theorem array_inv (lvl: Z) (head: node_rep) (t: loc)
       (bot: bot_gname) (subs: list sub_gname) (γ: gname):
       skip_list_equiv lvl head ∅ 1 bot subs
       ∗
-      is_lock γ (node_lock head) (node_inv (node_next head))
+      is_lock γ (node_lock head) (in_lock (node_next head))
       ∗
-      t ↦{#1 / exp2 (lvl + 1)} rep_to_node tail
+      inv (nodeN tail) (node_inv t tail)
       ∗
-      (node_next head +ₗ lvl +ₗ 1) ↦∗{#1 / 2} replicate (MAX_HEIGHT - lvl) #t 
+      (node_next head +ₗ lvl +ₗ 1) ↦∗{#1 / 2} replicate (Z.to_nat (MAX_HEIGHT - lvl)) #t 
       ∗
       ⌜ 0 ≤ lvl ≤ MAX_HEIGHT ⌝ 
       ∗
@@ -31,10 +33,10 @@ Module NewSpec (Params: SKIP_LIST_PARAMS).
         ∃ (subs: list sub_gname), 
           skip_list_equiv MAX_HEIGHT head ∅ 1 bot subs.
     Proof.
-      remember (MAX_HEIGHT - lvl) as diff eqn:Hdiff.
+      remember (Z.to_nat (MAX_HEIGHT - lvl)) as diff eqn:Hdiff.
       iRevert (lvl subs Hdiff).
       iInduction diff as [|d] "IHdiff";
-        iIntros (lvl subs Hdiff) "(Hlist & #Hlock & Ht & Hnext & %Hmax & %Hmin)".
+        iIntros (lvl subs Hdiff) "(Hlist & #Hlock & #Ht & Hnext & %Hmax & %Hmin)".
 
       + assert (lvl = MAX_HEIGHT) as -> by lia.
         iModIntro. iExists subs. iFrame.
@@ -42,7 +44,6 @@ Module NewSpec (Params: SKIP_LIST_PARAMS).
 
         rewrite replicate_S array_cons.
         iDestruct "Hnext" as "(Hnext' & Hnext)".
-        iDestruct "Ht" as "(Ht & Ht')".
 
         iMod (own_alloc (● (∅ : gset node_rep) ⋅ ◯ (∅: gset node_rep)))
           as (γauth) "[Hown_auth _]"; 
@@ -53,7 +54,7 @@ Module NewSpec (Params: SKIP_LIST_PARAMS).
 
         set (sub := mk_sub_gname γauth γtoks).
         iMod (inv_alloc (levelN (lvl + 1)) ⊤ (lazy_list_inv (lvl + 1) head sub None (from_top_list top_sub)) 
-          with "[Hnext' Ht' Hown_auth Hown_toks]") as "Hinv".
+          with "[Hnext' Hown_auth Hown_toks]") as "Hinv".
         {
           iNext; iExists ∅, ∅, nil. iFrame.
           iSplit; first done. iSplit.
@@ -63,12 +64,8 @@ Module NewSpec (Params: SKIP_LIST_PARAMS).
             rewrite /node_lt /node_key Hmin /=; apply HMIN_MAX.
           }
           iSplit; first rewrite /key_equiv //.
-          iExists γ, t. 
           rewrite loc_add_assoc.
-          assert (lvl + 1 + 1 = S (lvl + 1)) as -> by lia.
-          assert ((lvl + 1)%Z = lvl + 1) as -> by lia.
-          rewrite Qp_div_div comm_L //=.
-          iFrame "# ∗".
+          iExists γ, t. iFrame "# ∗".
         }
 
         iApply ("IHdiff" $! (lvl + 1) (sub :: top_sub :: bot_subs) with "[%]").
@@ -81,9 +78,6 @@ Module NewSpec (Params: SKIP_LIST_PARAMS).
           iFrame "# ∗". iPureIntro; lia.
         }
 
-        rewrite Qp_div_div comm_L //=.
-        assert (lvl + 1 + 1 = S (lvl + 1)) as -> by lia.
-        assert ((lvl + 1)%Z = lvl + 1) as <- by lia.
         rewrite -loc_add_assoc.
         iFrame "# ∗". iPureIntro.
         by split; first lia.
@@ -97,17 +91,22 @@ Module NewSpec (Params: SKIP_LIST_PARAMS).
       iIntros (Φ) "_ HΦ".
 
       wp_lam. wp_alloc t as "Ht". wp_let.
-      wp_alloc next as "Hnext"; first lia. wp_let.
-      assert (Z.to_nat (MAX_HEIGHT + 1) = S MAX_HEIGHT) as -> by lia.
+      iDestruct "Ht" as "(Ht & _)".
+      iMod (inv_alloc (nodeN tail) ⊤ (node_inv t tail) with "Ht") as "#Ht".
+
+      wp_alloc next as "Hnext".
+      { pose proof HMAX_HEIGHT; lia. } 
+      wp_let.
+      assert (Z.to_nat (MAX_HEIGHT + 1) = S (Z.to_nat MAX_HEIGHT)) as ->.
+      { pose proof HMAX_HEIGHT; lia. } 
       iDestruct "Hnext" as "(Hnext' & Hnext)".
 
-      wp_apply (newlock_spec (node_inv next) with "[Hnext']").
-      { iExists (replicate (S MAX_HEIGHT) #t); iFrame. }
+      wp_apply (newlock_spec (in_lock next) with "[Hnext']").
+      { iExists (replicate (S (Z.to_nat MAX_HEIGHT)) #t); iFrame. }
       iIntros (l) "#Hlock". iDestruct "Hlock" as (γ) "Hlock".
 
       rewrite replicate_S array_cons.
       iDestruct "Hnext" as "(Hnext' & Hnext)".
-      iDestruct "Ht" as "(Ht & Ht')".
 
       wp_pures.
       rewrite (fold_rep_to_node (INT_MIN, next, None, l)).
@@ -127,7 +126,7 @@ Module NewSpec (Params: SKIP_LIST_PARAMS).
       set (sub := mk_sub_gname γauth γtoks).
       set (bot := mk_bot_gname γfrac).
       iMod (inv_alloc (levelN 0) ⊤ (lazy_list_inv 0 head sub (Some bot) from_bot_list) 
-        with "[Hnext' Ht' Hown_auth Hown_toks Hown_frac]") as "Hinv".
+        with "[Hnext' Hown_auth Hown_toks Hown_frac]") as "Hinv".
       {
         iNext; iExists ∅, ∅, nil. iFrame.
         iSplit; first done. iSplit.
@@ -137,7 +136,7 @@ Module NewSpec (Params: SKIP_LIST_PARAMS).
         }
         iSplit; first rewrite /key_equiv //.
         iExists γ, t.
-        rewrite loc_add_0 /node_next /= Qp_mul_1_r.
+        rewrite loc_add_0 /node_next /=.
         iFrame "# ∗".
       }
 
@@ -147,11 +146,12 @@ Module NewSpec (Params: SKIP_LIST_PARAMS).
 
       iPoseProof (array_inv 0 head t bot [sub] γ with "[Hskip Hlock Ht Hnext]") as "Hskip".
       {
-        rewrite loc_add_assoc /node_next /= Qp_mul_1_r. 
-        assert (0%nat + 1 = 1)%Z as -> by lia.
+        rewrite loc_add_assoc /node_next /=. 
+        assert (0 + 1 = 1) as -> by lia.
         assert (MAX_HEIGHT - 0 = MAX_HEIGHT) as -> by lia.
         iFrame "# ∗". iPureIntro.
-        by split; first lia.
+        split; last done.
+        pose proof HMAX_HEIGHT; lia.
       }
       iMod "Hskip" as (subs) "Hskip".
 
