lazy_list/spec/add.v
@@ -34,7 +34,7 @@ Module AddSpec (Params: LAZY_LIST_PARAMS).
         ∗
         (own (s_auth Γ) (◯ {[succ]}) ∨ ⌜ succ = tail ⌝)
         ∗
-        ∃ (γ: gname), is_lock γ (node_lock pred) (node_inv (node_next pred))
+        ∃ (γ: gname), is_lock γ (node_lock pred) (in_lock (node_next pred))
       }}}.
     Proof.
       iIntros (Φ) "(#Hinv & Hown_curr & Hrange) HΦ".
@@ -113,7 +113,7 @@ Module AddSpec (Params: LAZY_LIST_PARAMS).
         ∗
         (own (s_auth Γ) (◯ {[succ]}) ∨ ⌜ succ = tail ⌝)
         ∗
-        ∃ (γ: gname), is_lock γ (node_lock pred) (node_inv (node_next pred))
+        ∃ (γ: gname), is_lock γ (node_lock pred) (in_lock (node_next pred))
                       ∗
                       node_next pred ↦{#1 / 2} rep_to_node succ
                       ∗
@@ -237,7 +237,7 @@ Module AddSpec (Params: LAZY_LIST_PARAMS).
         wp_alloc l as "Hpt'". wp_let.
         iDestruct "Hpt'" as "(Hpt' & Hpt'_dup)".
 
-        wp_apply (newlock_spec (node_inv l) with "[Hpt'_dup]").
+        wp_apply (newlock_spec (in_lock l) with "[Hpt'_dup]").
         { iExists succ; iFrame. }
         iIntros (lk) "#Hlock'". iDestruct "Hlock'" as (γ') "Hlock'".
 
